StaticMutrecBproof

demo/mutrec/StaticMutrecBproof.v
@@ -10,8 +10,9 @@ Require Import Simulation.
 Require Import Skeleton Mod ModSem SimMod SimModSem SimSymb SimMem AsmregsC MatchSimModSem.
 (* Require SimMemInjC. *)
 Require SoundTop.
-Require SimMemInjInvC.
-Require Import AsmC.
+Require SimMemInjInv SimMemInjInvC.
+Require Mach.
+Require Import AsmC AsmregsC Conventions1C MemoryC AsmExtra.
 
 Set Implicit Arguments.
 
@@ -93,17 +94,989 @@ Let md_src: Mod.t := (StaticMutrecBspec.module).
 Let md_tgt: Mod.t := (AsmC.module prog).
 Hypothesis (INCL: SkEnv.includes skenv_link md_src.(Mod.sk)).
 Hypothesis (WF: SkEnv.wf skenv_link).
-Let ge := (SkEnv.project skenv_link md_src.(Mod.sk)).
-Let tge := (SkEnv.project skenv_link md_tgt.(Mod.sk)).
+(* Let ge := (SkEnv.project skenv_link md_src.(Mod.sk)). *)
+(* Let tge := (SkEnv.revive (SkEnv.project skenv_link md_tgt.(Mod.sk)). *)
+
+Let tge := (skenv_link.(SkEnv.project) prog.(Sk.of_program fn_sig)).(SkEnv.revive) prog.
 Definition msp: ModSemPair.t :=
   ModSemPair.mk (md_src skenv_link) (md_tgt skenv_link) symbol_memoized sm_link.
+
+Inductive well_saved (initstk stk: block)
+  : regset -> regset -> mem -> Prop :=
+| well_saved_intro
+    (STKWF: initstk <> stk)
+    (init_rs rs: regset) m
+    (INITSIG: tge.(Genv.find_funct) (init_rs # PC) = Some (Internal func_g))
+    (INITRSPVAL: init_rs RSP = Vptr initstk Ptrofs.zero)
+    (RANOTFPTR: forall blk ofs (RAVAL: init_rs RA = Vptr blk ofs),
+        ~ Plt blk (Genv.genv_next skenv_link))
+    (RSPVAL: rs RSP = Vptr stk Ptrofs.zero)
+    (STKPERM: Mem.range_perm m stk 0 32 Cur Freeable)
+    (RASAVED: Mem.loadv Mptr m (Val.offset_ptr (rs RSP) (Ptrofs.repr 24)) = Some (init_rs RA))
+    (RSPSAVED: Mem.loadv Mptr m (Val.offset_ptr (rs RSP) Ptrofs.zero) = Some (init_rs RSP))
+    (REGSAVED: forall mr (CALLEESAVE: Conventions1.is_callee_save mr)
+                      (INREG: mr <> Machregs.BX), init_rs mr.(to_preg) = rs mr.(to_preg))
+    (REGSAVEDSTK: Mem.loadv Many64 m (Val.addl (rs RSP) (Vlong (Int64.repr 8))) = Some (init_rs RBX))
+  :
+    well_saved
+      initstk stk
+      init_rs rs m.
+
+Lemma well_saved_keep init_rs initstk stk rs0 rs1 m0 m1
+      (SAVED: well_saved
+                initstk stk
+                init_rs rs0 m0)
+      (REGSAME: forall mr (CALLEESAVE: Conventions1.is_callee_save mr)
+                       (INREG: mr <> Machregs.BX),
+          rs0 mr.(to_preg) = rs1 mr.(to_preg))
+      (RSPSAME: rs0 RSP = rs1 RSP)
+      (UNCHSTK: Mem.unchanged_on
+                   (fun blk _ => blk = stk) m0 m1)
+  :
+    well_saved
+      initstk stk
+      init_rs rs1 m1.
+Proof.
+  inv SAVED. rewrite RSPVAL in *. ss. econs; eauto.
+  - ii. eapply Mem.perm_unchanged_on; [apply UNCHSTK|..]; ss; eauto.
+  - rewrite <- RSPSAME. ss. erewrite Mem.load_unchanged_on; eauto. ss.
+  - rewrite <- RSPSAME. ss. erewrite Mem.load_unchanged_on; eauto. ss.
+  - ii. erewrite REGSAVED; eauto.
+  - ii. rewrite <- RSPSAME. ss. des_ifs. ss.
+    erewrite Mem.load_unchanged_on; eauto. ss.
+Qed.
+
+Inductive curr_pc (v: val) (ofs: ptrofs): Prop :=
+| curr_pc_intro
+    blk
+    (RSPC: v = Vptr blk ofs)
+    (FINDF: Genv.find_funct_ptr tge blk = Some (Internal func_g))
+.
+
+Require Import mktac.
+Require Import StoreArguments.
+
+
+(* TODO: from LB *)
+Lemma Mem_unchanged_on_strengthen P m0 m1
+  :
+    Mem.unchanged_on P m0 m1 <-> Mem.unchanged_on (SimMemInj.valid_blocks m0 /2\ P) m0 m1.
+Proof.
+  split; i.
+  - eapply Mem.unchanged_on_implies; eauto. i. des. auto.
+  - eapply Mem.unchanged_on_implies; eauto. ss.
+Qed.
+
+Inductive match_states (sm_init: SimMem.t)
+  :
+    nat -> StaticMutrecBspec.state -> AsmC.state -> SimMem.t -> Prop :=
+| match_states_initial
+    idx m_src sm0
+    i stk initstk init_rs rs m_tgt
+    (MCOMPATSRC: m_src = sm0.(SimMem.src))
+    (MCOMPATTGT: m_tgt = sm0.(SimMem.tgt))
+    (MWF: SimMem.wf sm0)
+    (MLE: SimMem.le sm_init sm0)
+    (SAVED: well_saved initstk stk init_rs rs m_tgt)
+    (OUTSIDE: forall
+        blk_src blk_tgt delta
+        (DETLA: SimMemInjInv.inj sm0 blk_src = Some (blk_tgt, delta)),
+        blk_tgt <> stk)
+    (CURRPC: curr_pc (rs PC) (Ptrofs.repr 2))
+    (ARG: rs RDI = Vint i)
+    (RANGE: 0 <= i.(Int.intval) < MAX)
+  :
+    match_states sm_init idx (Callstate i m_src)
+                 (AsmC.mkstate init_rs (Asm.State rs m_tgt)) sm0
+
+| match_states_at_external
+    idx m_src sm0
+    i stk initstk init_rs rs m_tgt
+    (MCOMPATSRC: m_src = sm0.(SimMem.src))
+    (MCOMPATTGT: m_tgt = sm0.(SimMem.tgt))
+    (MWF: SimMem.wf sm0)
+    (MLE: SimMem.le sm_init sm0)
+    (SAVED: well_saved initstk stk init_rs rs m_tgt)
+    (OUTSIDE: forall
+        blk_src blk_tgt delta
+        (DETLA: SimMemInjInv.inj sm0 blk_src = Some (blk_tgt, delta)),
+        blk_tgt <> stk)
+    (CURRPC: curr_pc (rs PC) (Ptrofs.repr 12))
+    (ARG: rs RBX = Vint i)
+    (FARG: rs RDI = Vint (Int.sub i (Int.repr 1)))
+  :
+    match_states sm_init idx (Interstate i m_src)
+                 (AsmC.mkstate init_rs (Asm.State rs m_tgt)) sm0
+
+| match_states_after_external
+    idx m_src sm0
+    i stk initstk init_rs rs m_tgt
+    (MCOMPATSRC: m_src = sm0.(SimMem.src))
+    (MCOMPATTGT: m_tgt = sm0.(SimMem.tgt))
+    (MWF: SimMem.wf sm0)
+    (MLE: SimMem.le sm_init sm0)
+    (SAVED: well_saved initstk stk init_rs rs m_tgt)
+    (OUTSIDE: forall
+        blk_src blk_tgt delta
+        (DETLA: SimMemInjInv.inj sm0 blk_src = Some (blk_tgt, delta)),
+        blk_tgt <> stk)
+    (CURRPC: curr_pc (rs PC) (Ptrofs.repr 13))
+    (ARG: rs RBX = Vint i)
+    (SUM: rs RAX = Vint (sum (Int.sub i Int.one)))
+  :
+    match_states sm_init idx (Returnstate (sum i) m_src)
+                 (AsmC.mkstate init_rs (Asm.State rs m_tgt))sm0
+
+| match_states_final
+    idx m_src sm0
+    i stk initstk init_rs rs m_tgt
+    (MCOMPATSRC: m_src = sm0.(SimMem.src))
+    (MCOMPATTGT: m_tgt = sm0.(SimMem.tgt))
+    (MWF: SimMem.wf sm0)
+    (MLE: SimMem.le sm_init sm0)
+    (SAVED: well_saved initstk stk init_rs rs m_tgt)
+    (OUTSIDE: forall
+        blk_src blk_tgt delta
+        (DETLA: SimMemInjInv.inj sm0 blk_src = Some (blk_tgt, delta)),
+        blk_tgt <> stk)
+    (CURRPC: curr_pc (rs PC) (Ptrofs.repr 20))
+    (ARG: rs RAX = Vint i)
+  :
+    match_states sm_init idx (Returnstate i m_src)
+                 (AsmC.mkstate init_rs (Asm.State rs m_tgt)) sm0
+.
+
+(* TODO: from DempProof *)
+Lemma E0_double:
+  E0 = E0 ** E0.
+Proof. auto. Qed.
+Hint Resolve E0_double.
+
+Lemma match_states_lxsim
+      sm_init idx st_src0 st_tgt0 sm0
+      (SIMSK: SimSymb.sim_skenv
+                sm0 symbol_memoized
+                (SkEnv.project skenv_link (Sk.of_program fn_sig prog))
+                (SkEnv.project skenv_link (Sk.of_program fn_sig prog)))
+      (MATCH: match_states sm_init idx st_src0 st_tgt0 sm0)
+  :
+    <<XSIM: lxsim (md_src skenv_link) (md_tgt skenv_link)
+                  (fun st => unit -> exists su m_init, SoundTop.sound_state su m_init st)
+                  sm_init (Ord.lift_idx lt_wf idx) st_src0 st_tgt0 sm0>>
+.
+Proof.
+  destruct (Genv.find_symbol
+              ((skenv_link.(SkEnv.project) prog.(Sk.of_program fn_sig)).(SkEnv.revive) prog)
+              _memoized) as [b_memo|] eqn:BLK; cycle 1.
+  { exfalso. clear - INCL BLK. inv INCL.
+    exploit DEFS; eauto.
+    - instantiate (2:=_memoized). ss.
+    - i. des. admit "genv". }
+
+  revert_until tge.
+  pcofix CIH.
+  i. pfold. inv MATCH.
+
+
+
+  (* initial *)
+  - intros _. inv CURRPC.
+
+    assert (CMP: compare_ints
+                   (Val.and (rs RDI) (rs RDI)) Vzero
+                   (rs # RBX <- (rs RDI)) # PC <- (Vptr blk (Ptrofs.add (Ptrofs.repr 2) Ptrofs.one))
+                   (SimMemInjInv.tgt sm0) ZF = if (Int.eq_dec i Int.zero) then Vtrue else Vfalse).
+    { unfold compare_ints, nextinstr, Val.cmpu.
+      repeat (rewrite Pregmap.gso; [| clarify; fail]).
+      repeat rewrite Pregmap.gss.
+      rewrite ARG. ss. rewrite Int.and_idem.
+      exploit Int.eq_spec; eauto. i. des_ifs. }
+    destruct (classic (i = Int.zero)).
+
+    (* i = Int.zero *)
+    + clarify. econs 1. i. econs.
+      * admit "ez".
+      * i. ss. inv STEPSRC; ss.
+
+        esplits.
+        {
+          left. econs; eauto.
+          { instantiate (1:=AsmC.mkstate _ _). split.
+            - eapply modsem_determinate; eauto.
+            - ss. econs; ss. econs; eauto.
+              + des_ifs.
+              + ss. }
+
+          econs 2; eauto.
+          { instantiate (1:=AsmC.mkstate _ _). split.
+            - eapply modsem_determinate; eauto.
+            - ss. econs; ss. econs; eauto.
+              + unfold nextinstr.
+                rewrite Pregmap.gss.
+                rewrite Pregmap.gso; clarify.
+                rewrite RSPC. ss.
+              + des_ifs.
+              + ss. }
+
+          econs 2; eauto.
+          { instantiate (1:=AsmC.mkstate _ _). split.
+            - eapply modsem_determinate; eauto.
+            - ss. econs; ss. econs; eauto.
+              + unfold nextinstr.
+                repeat rewrite Pregmap.gss.
+                repeat (rewrite Pregmap.gso; [| clarify; fail]).
+                repeat rewrite Pregmap.gss.
+                repeat (rewrite Pregmap.gso; [| clarify; fail]).
+                rewrite RSPC. ss.
+              + des_ifs.
+              + ss.
+                unfold nextinstr.
+                repeat rewrite Pregmap.gss.
+                repeat (rewrite Pregmap.gso; [| clarify; fail]).
+                repeat rewrite Pregmap.gss.
+                repeat (rewrite Pregmap.gso; [| clarify; fail]).
+                rewrite RSPC. ss. rewrite CMP. ss. }
+
+          econs 2; eauto.
+          { instantiate (1:=AsmC.mkstate _ _). split.
+            - eapply modsem_determinate; eauto.
+            - ss. econs; ss. econs; eauto.
+              + unfold nextinstr.
+                rewrite Pregmap.gss. ss.
+              + des_ifs.
+              + ss. }
+
+          econs 2; eauto.
+          { instantiate (1:=AsmC.mkstate _ _). split.
+            - eapply modsem_determinate; eauto.
+            - ss. econs; ss. econs; eauto.
+              + unfold nextinstr_nf, undef_regs, nextinstr. ss.
+              + des_ifs.
+              + ss. }
+
+          econs 1.
+        }
+
+        { refl. }
+
+        { right. eapply CIH; eauto. econs 4; eauto.
+
+          - eapply well_saved_keep; eauto.
+            + admit "ez".
+            + refl.
+
+          - ss.
+            unfold nextinstr_nf, nextinstr, undef_regs.
+            repeat rewrite Pregmap.gss. econs; eauto.
+
+          - ss.
+            unfold nextinstr_nf, nextinstr, undef_regs.
+            repeat (rewrite Pregmap.gso; [| clarify; fail]).
+            repeat rewrite Pregmap.gss.
+            admit "arithemetic". }
+
+      * admit "spec receptive".
+
+    (* i <> Int.zero *)
+    +
+
+      cinv MWF. ss.
+      assert (INVAR: SimMemInjInv.mem_inv sm0 b_memo).
+      { inv SIMSK. ss. inv INJECT.
+        eapply INVCOMPAT; eauto. ss. }
+      hexploit SAT; eauto. intros SAT0.
+      specialize (SAT0 _ INVAR). destruct SAT0. des. des_ifs_safe.
+
+      assert (CMP0:
+                nextinstr
+                  (compare_ints
+                     (nextinstr_nf
+                        (((compare_ints (Val.and (rs RDI) (rs RDI)) Vzero
+                                        (rs # RBX <- (rs RDI)) # PC <-
+                                        (Vptr blk (Ptrofs.add (Ptrofs.repr 2) Ptrofs.one))
+                                        (SimMemInjInv.tgt sm0)) # PC <-
+                                                                (Vptr blk (Ptrofs.add (Ptrofs.add (Ptrofs.repr 2) Ptrofs.one) Ptrofs.one)))
+                           # PC <- (Vptr blk (Ptrofs.repr 8))) # RAX <- (Vint x) RBX)
+                     (nextinstr_nf
+                        (((compare_ints (Val.and (rs RDI) (rs RDI)) Vzero
+                                        (rs # RBX <- (rs RDI)) # PC <-
+                                        (Vptr blk (Ptrofs.add (Ptrofs.repr 2) Ptrofs.one))
+                                        (SimMemInjInv.tgt sm0)) # PC <-
+                                                                (Vptr blk (Ptrofs.add (Ptrofs.add (Ptrofs.repr 2) Ptrofs.one) Ptrofs.one)))
+                           # PC <- (Vptr blk (Ptrofs.repr 8))) # RAX <- (Vint x) RAX)
+                     (nextinstr_nf
+                        (((compare_ints (Val.and (rs RDI) (rs RDI)) Vzero
+                                        (rs # RBX <- (rs RDI)) # PC <-
+                                        (Vptr blk (Ptrofs.add (Ptrofs.repr 2) Ptrofs.one))
+                                        (SimMemInjInv.tgt sm0)) # PC <-
+                                                                (Vptr blk (Ptrofs.add (Ptrofs.add (Ptrofs.repr 2) Ptrofs.one) Ptrofs.one)))
+                           # PC <- (Vptr blk (Ptrofs.repr 8))) # RAX <- (Vint x))
+                     (SimMemInjInv.tgt sm0)) ZF =
+                if (Int.eq_dec x i) then Vtrue else Vfalse).
+      { unfold compare_ints at 1.
+        unfold nextinstr_nf, undef_regs, nextinstr.
+        repeat (rewrite Pregmap.gso; [| clarify; fail]).
+        repeat rewrite Pregmap.gss. ss.
+        repeat (rewrite Pregmap.gso; [| clarify; fail]).
+        repeat rewrite Pregmap.gss. ss.
+        unfold Val.cmpu, Val.of_optbool, Val.cmpu_bool. ss.
+        unfold compare_ints.
+        repeat (rewrite Pregmap.gso; [| clarify; fail]).
+        repeat rewrite Pregmap.gss.
+        rewrite ARG.
+        exploit Int.eq_spec; eauto. i. des_ifs. }
+
+      destruct (Int.eq_dec x i).
+
+      (* already memoized *)
+      { clarify. econs 2. i. splits.
+        - econs 2.
+          + split.
+            * apply star_one. ss. econs 1.
+            * admit "index".
+          + refl.
+          + left. pfold. intros _. econs 1. i. econs 2.
+
+            * esplits.
+              {
+                econs; eauto.
+                { instantiate (1:=AsmC.mkstate _ _). split.
+                  - eapply modsem_determinate; eauto.
+                  - ss. econs; ss. econs; eauto.
+                    + des_ifs.
+                    + ss. }
+
+                econs 2; eauto.
+                { instantiate (1:=AsmC.mkstate _ _). split.
+                  - eapply modsem_determinate; eauto.
+                  - ss. econs; ss. econs; eauto.
+                    + unfold nextinstr.
+                      rewrite Pregmap.gss.
+                      rewrite Pregmap.gso; clarify.
+                      rewrite RSPC. ss.
+                    + des_ifs.
+                    + ss. }
+
+                econs 2; eauto.
+                { instantiate (1:=AsmC.mkstate _ _). split.
+                  - eapply modsem_determinate; eauto.
+                  - ss. econs; ss. econs; eauto.
+                    + unfold nextinstr.
+                      repeat rewrite Pregmap.gss.
+                      repeat (rewrite Pregmap.gso; [| clarify; fail]).
+                      repeat rewrite Pregmap.gss.
+                      repeat (rewrite Pregmap.gso; [| clarify; fail]).
+                      rewrite RSPC. ss.
+                    + des_ifs.
+                    + ss.
+                      unfold nextinstr.
+                      repeat rewrite Pregmap.gss.
+                      repeat (rewrite Pregmap.gso; [| clarify; fail]).
+                      repeat rewrite Pregmap.gss.
+                      repeat (rewrite Pregmap.gso; [| clarify; fail]).
+                      rewrite RSPC. ss. rewrite CMP.
+                      simpl.
+                      des_ifs. }
+
+                econs 2; eauto.
+                { instantiate (1:=AsmC.mkstate _ _). split.
+                  - eapply modsem_determinate; eauto.
+                  - ss. econs; ss. econs; eauto.
+                    + unfold nextinstr.
+                      repeat rewrite Pregmap.gss. ss.
+                    + des_ifs.
+                    + ss. unfold exec_load, eval_addrmode. ss.
+                      unfold Genv.symbol_address. ss. rewrite BLK. psimpl.
+                      des_ifs_safe. ss. psimpl.
+                      replace (Ptrofs.unsigned (Ptrofs.of_int64 Int64.zero)) with 0; cycle 1.
+                      { admit "arithmetic". }
+                      rewrite VINDEX. ss. }
+
+                econs 2; eauto.
+                { instantiate (1:=AsmC.mkstate _ _). split.
+                  - eapply modsem_determinate; eauto.
+                  - ss. econs; ss. econs; eauto.
+                    + unfold nextinstr_nf, undef_regs, nextinstr.
+                      repeat rewrite Pregmap.gss. ss.
+                    + des_ifs.
+                    + ss. }
+
+                econs 2; eauto.
+                { instantiate (1:=AsmC.mkstate _ _). split.
+                  - eapply modsem_determinate; eauto.
+                  - ss. econs; ss. econs; eauto.
+                    + unfold nextinstr_nf, undef_regs, nextinstr.
+                      repeat rewrite Pregmap.gss. ss.
+                    + des_ifs.
+                    + ss. rewrite CMP0. ss. }
+
+                econs 2; eauto.
+                { instantiate (1:=AsmC.mkstate _ _). split.
+                  - eapply modsem_determinate; eauto.
+                  - ss. econs; ss. econs; eauto.
+                    + unfold nextinstr.
+                      repeat rewrite Pregmap.gss. ss.
+                    + des_ifs.
+                    + ss. unfold exec_load, eval_addrmode. ss.
+                      unfold Genv.symbol_address. ss. rewrite BLK. psimpl.
+                      des_ifs_safe. ss.
+                      replace (Ptrofs.unsigned (Ptrofs.add (Ptrofs.repr 4) (Ptrofs.of_int64 Int64.zero))) with 4; cycle 1.
+                      { admit "arithmetic". }
+                      rewrite VSUM. ss. }
+
+                econs 2; eauto.
+                { instantiate (1:=AsmC.mkstate _ _). split.
+                  - eapply modsem_determinate; eauto.
+                  - ss. econs; ss. econs; eauto.
+                    + unfold nextinstr.
+                      repeat rewrite Pregmap.gss. ss.
+                    + des_ifs.
+                    + ss. }
+
+                econs 1.
+              }
+
+              { admit "index". }
+
+            * refl.
+
+            * right. eapply CIH; eauto.
+              econs 4; eauto.
+              { eapply well_saved_keep; eauto.
+                - admit "ez".
+                - refl. }
+              { unfold nextinstr_nf, nextinstr.
+                repeat rewrite Pregmap.gss. ss. econs; eauto. }
+
+        - admit "safe". }
+
+      (* not memoized *)
+      { clarify. econs 2. i. splits.
+        - econs 2.
+          + split.
+            * apply star_one. ss. econs 2.
+              admit "arithmetic".
+            * admit "index".
+          + refl.
+          + left. pfold. intros _. econs 1. i. econs 2.
+
+            * esplits.
+              {
+                econs; eauto.
+                { instantiate (1:=AsmC.mkstate _ _). split.
+                  - eapply modsem_determinate; eauto.
+                  - ss. econs; ss. econs; eauto.
+                    + des_ifs.
+                    + ss. }
+
+                econs 2; eauto.
+                { instantiate (1:=AsmC.mkstate _ _). split.
+                  - eapply modsem_determinate; eauto.
+                  - ss. econs; ss. econs; eauto.
+                    + unfold nextinstr.
+                      rewrite Pregmap.gss.
+                      rewrite Pregmap.gso; clarify.
+                      rewrite RSPC. ss.
+                    + des_ifs.
+                    + ss. }
+
+                econs 2; eauto.
+                { instantiate (1:=AsmC.mkstate _ _). split.
+                  - eapply modsem_determinate; eauto.
+                  - ss. econs; ss. econs; eauto.
+                    + unfold nextinstr.
+                      repeat rewrite Pregmap.gss.
+                      repeat (rewrite Pregmap.gso; [| clarify; fail]).
+                      repeat rewrite Pregmap.gss.
+                      repeat (rewrite Pregmap.gso; [| clarify; fail]).
+                      rewrite RSPC. ss.
+                    + des_ifs.
+                    + ss.
+                      unfold nextinstr.
+                      repeat rewrite Pregmap.gss.
+                      repeat (rewrite Pregmap.gso; [| clarify; fail]).
+                      repeat rewrite Pregmap.gss.
+                      repeat (rewrite Pregmap.gso; [| clarify; fail]).
+                      rewrite RSPC. ss. rewrite CMP.
+                      simpl.
+                      des_ifs. }
+
+                econs 2; eauto.
+                { instantiate (1:=AsmC.mkstate _ _). split.
+                  - eapply modsem_determinate; eauto.
+                  - ss. econs; ss. econs; eauto.
+                    + unfold nextinstr.
+                      repeat rewrite Pregmap.gss. ss.
+                    + des_ifs.
+                    + ss. unfold exec_load, eval_addrmode. ss.
+                      unfold Genv.symbol_address. ss. rewrite BLK. psimpl.
+                      des_ifs_safe. ss. psimpl.
+                      replace (Ptrofs.unsigned (Ptrofs.of_int64 Int64.zero)) with 0; cycle 1.
+                      { admit "arithmetic". }
+                      rewrite VINDEX. ss. }
+
+                econs 2; eauto.
+                { instantiate (1:=AsmC.mkstate _ _). split.
+                  - eapply modsem_determinate; eauto.
+                  - ss. econs; ss. econs; eauto.
+                    + unfold nextinstr_nf, undef_regs, nextinstr.
+                      repeat rewrite Pregmap.gss. ss.
+                    + des_ifs.
+                    + ss. }
+
+                econs 2; eauto.
+                { instantiate (1:=AsmC.mkstate _ _). split.
+                  - eapply modsem_determinate; eauto.
+                  - ss. econs; ss. econs; eauto.
+                    + unfold nextinstr_nf, undef_regs, nextinstr.
+                      repeat rewrite Pregmap.gss. ss.
+                    + des_ifs.
+                    + ss. rewrite CMP0. ss. }
+
+                econs 2; eauto.
+                { instantiate (1:=AsmC.mkstate _ _). split.
+                  - eapply modsem_determinate; eauto.
+                  - ss. econs; ss. econs; eauto.
+                    + unfold nextinstr.
+                      repeat rewrite Pregmap.gss. ss.
+                    + des_ifs.
+                    + ss. }
+
+                econs 1.
+              }
+
+              { admit "index". }
+
+            * refl.
+
+            * right. eapply CIH; eauto.
+              econs 2; eauto.
+              { eapply well_saved_keep; eauto.
+                - admit "ez".
+                - refl. }
+              { unfold nextinstr_nf, nextinstr.
+                repeat rewrite Pregmap.gss. ss. econs; eauto. }
+              { unfold nextinstr_nf, nextinstr.
+                repeat rewrite Pregmap.gss.
+                repeat (rewrite Pregmap.gso; [| clarify; fail]). ss.
+                repeat rewrite Pregmap.gss.
+                repeat (rewrite Pregmap.gso; [| clarify; fail]). ss.
+                repeat rewrite Pregmap.gss.
+                unfold compare_ints.
+                repeat (rewrite Pregmap.gso; [| clarify; fail]). ss.
+                repeat rewrite Pregmap.gss.
+                rewrite ARG. ss. f_equal.
+                admit "arithmetic". }
+
+        - admit "safe".
+      }
+
+  - intros _. inv CURRPC.
+    econs 1. i. econs 2.
+    { split.
+      - instantiate (1:=AsmC.mkstate _ _). apply plus_one. split.
+        + eapply modsem_determinate; eauto.
+        + ss. econs; ss. econs; eauto.
+          * des_ifs.
+          * ss.
+      - admit "index". }
+    { refl. }
+
+    left. pfold. intros _. econs 3; eauto.
+    + econs; eauto. econs; eauto.
+      instantiate (1:=g_id). admit "genv".
+    + ii.
+
+      hexploit Mem.range_perm_free.
+      { instantiate (1:=0).
+        instantiate (1:=0).
+        instantiate (1:=stk).
+        instantiate (1:=SimMem.tgt sm0).
+        ii. lia. } intros [m_tgt FREE].
+
+
+      cinv MWF.
+      hexploit (@SimMemInjInv.unchanged_on_mle
+                  memoized_inv sm0
+                  sm0.(SimMemInjInv.src) m_tgt sm0.(SimMemInjInv.inj)); ss; eauto.
+      { eapply private_unchanged_inject; eauto.
+        - eapply Mem.free_unchanged_on; eauto. ii. omega.
+        - instantiate (1:=~2 loc_out_of_reach (SimMemInjInv.inj sm0) (SimMemInjInv.src sm0)).
+          ss.
+        - symmetry. eapply Mem.nextblock_free; eauto. }
+      { ii. clarify. }
+      { refl. }
+      { eapply Mem.free_unchanged_on; eauto. ii. omega. }
+      { ii. eapply Mem.perm_free_3; eauto. }
+      i. des.
+
+      cinv SAVED. inv ATSRC.
+      eexists (Args.mk _ [Vint (Int.sub i (Int.repr 1))] _).
+      esplits; eauto.
+      * econs; ss; eauto.
+        admit "genv".
+      * econs; eauto.
+        { repeat rewrite Pregmap.gss. ss.
+          instantiate (1:=g_fptr).
+          admit "genv". }
+        { admit "genv". }
+        { instantiate (1:=(mksignature (AST.Tint :: nil) (Some AST.Tint) cc_default)).
+          admit "genv". }
+        { unfold size_arguments. des_ifs. }
+        { econs; eauto.
+          - econs; eauto. ss.
+            rpapply extcall_arg_reg. ss.
+          - econs. }
+        { split; ss.
+          - repeat (rewrite Pregmap.gso; [| clarify; fail]).
+            rewrite Pregmap.gss. rewrite RSPC. ss.
+          - repeat (rewrite Pregmap.gso; [| clarify; fail]).
+            rewrite Pregmap.gss. rewrite RSPC. ss. }
+        { ii. apply Z.divide_0_r. }
+        { eauto. }
+
+      * i. inv SIMRETV. inv AFTERSRC. ss.
+        exploit Mem_unfree_suceeds.
+        { instantiate (1:=stk).
+          instantiate (1:=SimMemInjInv.tgt sm_ret).
+          admit "ez". } i. des.
+        eexists.
+        eexists (SimMemInjInv.mk
+                   (SimMemInjInv.src sm_ret)
+                   m1
+                   (SimMemInjInv.inj sm_ret)
+                   (SimMemInjInv.mem_inv sm_ret)).
+        eexists. esplits; ss; eauto.
+
+        { econs; ss; eauto.
+          - instantiate (1:=mksignature (AST.Tint :: nil) (Some AST.Tint) cc_default).
+            admit "genv".
+          - unfold size_arguments. des_ifs. ss. psimpl.
+            rewrite MEMTGT. eauto. }
+        { admit "make lemma". }
+
+        { right. eapply CIH; eauto.
+          { admit "find lemma". }
+          econs 3; ss; eauto.
+          - admit "make lemma".
+          - admit "make lemma".
+          - eapply well_saved_keep; eauto.
+            + admit "ez".
+            + admit "ez".
+          - admit "ez".
+          - repeat rewrite Pregmap.gss. rewrite RSPC.
+            repeat (rewrite Pregmap.gso; [| clarify; fail]).
+            repeat rewrite Pregmap.gss. ss. econs; eauto.
+          - unfold set_pair, loc_external_result, loc_result. des_ifs_safe. ss.
+            clarify.
+            repeat (rewrite Pregmap.gso; [| clarify; fail]).
+            repeat rewrite Pregmap.gss.
+            rewrite INT in *. inv RETV. auto. }
+
+  - intros _. econs 1. i. cinv CURRPC.
+
+    cinv MWF. ss.
+    assert (INVAR: SimMemInjInv.mem_inv sm0 b_memo).
+    { inv SIMSK. ss. inv INJECT.
+      eapply INVCOMPAT; eauto. ss. }
+    hexploit SAT; eauto. intros SAT0.
+    specialize (SAT0 _ INVAR). destruct SAT0. des. des_ifs_safe.
+
+    hexploit Mem.valid_access_store.
+    { eapply v0. } intros [m_tgt0 STR0].
+    hexploit Mem.valid_access_store.
+    { eapply Mem.store_valid_access_1; eauto. } intros [m_tgt1 STR1].
+
+    hexploit memoized_inv_store_le; try refl; eauto.
+    instantiate (1:=i) in STR0. i. des.
+
+    econs 2.
+
+    + split.
+      * econs 1; eauto.
+        { instantiate (1:=AsmC.mkstate _ _). split.
+          - eapply modsem_determinate; eauto.
+          - ss. econs; ss. econs; eauto.
+            + des_ifs.
+            + ss. }
+
+        econs 2; eauto.
+        { instantiate (1:=AsmC.mkstate _ _). split.
+          - eapply modsem_determinate; eauto.
+          - ss. econs; ss. econs; eauto.
+            + unfold nextinstr.
+              repeat rewrite Pregmap.gss.
+              repeat (rewrite Pregmap.gso; [| clarify; fail]).
+              rewrite RSPC. ss.
+            + des_ifs.
+            + ss.
+              unfold exec_store, Mem.storev, eval_addrmode. ss.
+              des_ifs_safe. unfold Genv.symbol_address. rewrite BLK.
+              psimpl. unfold nextinstr at 1.
+              repeat (rewrite Pregmap.gso; [| clarify; fail]).
+              rewrite ARG.
+              replace (Ptrofs.unsigned (Ptrofs.of_int64 Int64.zero)) with 0; cycle 1.
+              { admit "arithmetic". }
+              rewrite STR0.
+              ss. }
+
+        econs 2; eauto.
+        { instantiate (1:=AsmC.mkstate _ _). split.
+          - eapply modsem_determinate; eauto.
+          - ss. econs; ss. econs; eauto.
+            + unfold nextinstr_nf, undef_regs, nextinstr.
+              repeat rewrite Pregmap.gss.
+              repeat (rewrite Pregmap.gso; [| clarify; fail]).
+              repeat rewrite Pregmap.gss.
+              repeat (rewrite Pregmap.gso; [| clarify; fail]).
+              rewrite RSPC. ss.
+            + des_ifs.
+            + ss.
+              unfold exec_store, Mem.storev, eval_addrmode. ss.
+              des_ifs_safe. unfold Genv.symbol_address. rewrite BLK.
+              psimpl. unfold nextinstr_nf at 1.
+              unfold undef_regs. unfold nextinstr at 1 2.
+              repeat (rewrite Pregmap.gso; [| clarify; fail]).
+              repeat rewrite Pregmap.gss. rewrite SUM.
+              replace
+                (Val.add (Vint (sum (Int.sub i Int.one))) (Vint (Int.add i (Int.repr 0))))
+                with (Vint (sum i)); cycle 1.
+              { admit "arithmetic". }
+              rewrite STR1. ss. }
+
+        econs 2; eauto.
+        { instantiate (1:=AsmC.mkstate _ _). split.
+          - eapply modsem_determinate; eauto.
+          - ss. econs; ss. econs; eauto.
+            + unfold nextinstr_nf, undef_regs, nextinstr.
+              repeat rewrite Pregmap.gss.
+              repeat (rewrite Pregmap.gso; [| clarify; fail]).
+              repeat rewrite Pregmap.gss.
+              repeat (rewrite Pregmap.gso; [| clarify; fail]).
+              repeat rewrite Pregmap.gss.
+              repeat (rewrite Pregmap.gso; [| clarify; fail]).
+              rewrite RSPC. ss.
+            + des_ifs.
+            + ss. unfold goto_label.
+              unfold nextinstr_nf, undef_regs, nextinstr.
+              repeat rewrite Pregmap.gss.
+              repeat (rewrite Pregmap.gso; [| clarify; fail]).
+              repeat rewrite Pregmap.gss.
+              repeat (rewrite Pregmap.gso; [| clarify; fail]).
+              repeat rewrite Pregmap.gss.
+              repeat (rewrite Pregmap.gso; [| clarify; fail]).
+              rewrite RSPC. ss. }
+
+        econs 1; eauto.
+
+      * admit "index".
+
+    + eauto.
+
+    + right. eapply CIH; eauto.
+      { admit "ez". }
+      econs 4; ss; eauto.
+
+      * etrans; eauto.
+
+      * eapply well_saved_keep; eauto.
+        { admit "ez". }
+        { admit "ez". }
+
+      * repeat rewrite Pregmap.gss. econs; eauto.
+
+
+  - admit "see well_saved final".
+
+    Unshelve. all:admit"".
+Qed.
+
+(* Lemma well_saved_initial init_rs rs0 m0 arg *)
+(*       (INITIAL: initial_frame *)
+(*                   skenv_link prog arg *)
+(*                   (AsmC.mkstate init_rs (Asm.State rs0 m0))) *)
+(*   : *)
+(*     exists fd initstk stk rs1 m1 rs2 m2, *)
+(*       (<<ALLOCFRAME: exec_instr *)
+(*                        tge fd (Pallocframe 32 (Ptrofs.repr 24) (Ptrofs.zero)) rs0 m0 = Next rs1 m1>>) /\ *)
+(*       (<<PUSH: exec_instr *)
+(*                  tge func_g *)
+(*                  (Pmov_mr_a (Addrmode (Some RSP) None (inl 8)) RBX) *)
+(*                  rs1 m1 = Next rs2 m2>>) /\ *)
+(*       (<<SAVED: well_saved *)
+(*                   initstk stk *)
+(*                   (AsmC.mkstate init_rs (Asm.State rs2 m2))>>) *)
+(* . *)
+(* (* TODO: about fd and arguments, pc *) *)
+(* (* TODO: about memory *) *)
+(* Proof. *)
+(*   inv INITIAL. cinv STORE. des. *)
+(*   ss. destruct (Mem.alloc (JunkBlock.assign_junk_blocks m1 n) 0 32) as [m2 stk] eqn:ALLOC. *)
+(*   hexploit Mem.valid_access_store. *)
+(*   { eapply Mem.valid_access_implies. *)
+(*     - instantiate (4:=Mptr). *)
+(*       eapply Mem.valid_access_alloc_same. *)
+(*       + eauto. *)
+(*       + instantiate (1:=Ptrofs.unsigned Ptrofs.zero). ss. *)
+(*       + unfold Mptr. des_ifs. *)
+(*       + apply Z.divide_0_r. *)
+(*     - econs. } intros [m3 STR0]. *)
+(*   psimpl. rewrite STR0. *)
+(*   hexploit Mem.valid_access_store. *)
+(*   { eapply Mem.valid_access_implies. *)
+(*     - instantiate (4:=Mptr). *)
+(*       eapply Mem.store_valid_access_1; eauto. *)
+(*       eapply Mem.valid_access_alloc_same. *)
+(*       + eauto. *)
+(*       + instantiate (1:=Ptrofs.unsigned (Ptrofs.repr 24)). ss. *)
+(*       + unfold Mptr. des_ifs. *)
+(*       + rewrite align_chunk_Mptr. des_ifs. exists 3. ss. *)
+(*     - econs. } intros [m4 STR1]. rewrite STR1. *)
+(*   unfold exec_store, eval_addrmode, eval_addrmode64. des_ifs_safe. ss. *)
+(*   hexploit Mem.valid_access_store. *)
+(*   { eapply Mem.valid_access_implies. *)
+(*     - instantiate (4:=Many64). *)
+(*       eapply Mem.store_valid_access_1; eauto. *)
+(*       eapply Mem.store_valid_access_1; eauto. *)
+(*       eapply Mem.valid_access_alloc_same. *)
+(*       + eauto. *)
+(*       + instantiate (1:=Ptrofs.unsigned (Ptrofs.repr 8)). ss. *)
+(*       + unfold Mptr. des_ifs. *)
+(*       + ss. exists 2. auto. *)
+(*     - econs. } intros [m5 STR2]. *)
+(*   esplits; eauto. ss. des_ifs_safe. ss. *)
+
+(*   - unfold Ptrofs.of_int64. psimpl. rewrite Int64.add_zero_l. *)
+(*     rewrite STR2. eauto. *)
+(*   - econs; ss; eauto. *)
+
+(*     + eapply Mem.alloc_result in ALLOC. clarify. ii. *)
+(*       cinv H0. eapply Mem.nextblock_alloc in ALC. rewrite ALC in NB. *)
+(*       clear - NB H. *)
+(*       exploit JunkBlock.assign_junk_blocks_unchanged_on. *)
+(*       instantiate (1:=n). instantiate (1:=m1). i. *)
+(*       eapply Mem.unchanged_on_nextblock in H0. *)
+(*       rewrite <- NB in *. rewrite <- H in *. clear - H0. xomega. *)
+
+(*     + admit "genv". *)
+
+(*     + ii. *)
+(*       eapply Mem.perm_store_1; eauto. *)
+(*       eapply Mem.perm_store_1; eauto. *)
+(*       eapply Mem.perm_store_1; eauto. *)
+(*       eapply Mem.perm_alloc_2; eauto. *)
+
+(*     + psimpl. erewrite Mem.load_store_other; eauto; cycle 1. *)
+(*       { rewrite size_chunk_Mptr. des_ifs. ss. right. lia. } *)
+(*       erewrite Mem.load_store_same; eauto. *)
+(*       f_equal. erewrite <- Val.load_result_same; eauto. ss. *)
+
+(*     + psimpl. erewrite Mem.load_store_other; eauto; cycle 1. *)
+(*       { rewrite size_chunk_Mptr. des_ifs. ss. right. lia. } *)
+(*       erewrite Mem.load_store_other; eauto; cycle 1. *)
+(*       { rewrite size_chunk_Mptr. des_ifs. ss. right. lia. } *)
+(*       erewrite Mem.load_store_same; eauto. *)
+(*       f_equal. rewrite H1. ss. *)
+
+(*     + i. unfold nextinstr_nf, nextinstr, undef_regs, to_preg, preg_of, Pregmap.set. *)
+(*       des_ifs. *)
+
+(*     + des_ifs. unfold Ptrofs.of_int64. psimpl. *)
+(*       unfold nextinstr in STR2. *)
+(*       repeat (rewrite Pregmap.gso in STR2; clarify). *)
+(*       erewrite Mem.load_store_same; eauto. ss. *)
+(* Qed. *)
+
+(* Lemma well_saved_final initstk stk init_rs rs0 m0 *)
+(*       (SAVED: well_saved *)
+(*                 initstk stk *)
+(*                 (AsmC.mkstate init_rs (Asm.State rs0 m0))) *)
+(*   : *)
+(*     exists rs1 rs2 rs3 m2 m4, *)
+(*       (<<POP: exec_instr *)
+(*                 tge func_g (Pmov_rm_a RBX (Addrmode (Some RSP) None (inl 8))) *)
+(*                 rs0 m0 = Next rs1 m0>>) /\ *)
+(*       (<<FREEFRAME: exec_instr *)
+(*                       tge func_g (Pfreeframe 32 (Ptrofs.repr 24) Ptrofs.zero) rs1 m0 = Next rs2 m2>>) /\ *)
+(*       (<<RET: exec_instr *)
+(*                 tge func_g Pret rs2 m2 = Next rs3 m2>>) /\ *)
+(*       (<<FREE: Mem.free m2 initstk 0 0 = Some m4>>) /\ *)
+(*       (<<FINAL: final_frame *)
+(*                   skenv_link prog *)
+(*                   (AsmC.mkstate init_rs (Asm.State rs3 m2)) *)
+(*                   (Retv.mk (rs0 RAX) m4) >>). *)
+(* Proof. *)
+(*   inv SAVED. ss. *)
+(*   unfold exec_load, eval_addrmode, eval_addrmode64. des_ifs_safe. ss. *)
+(*   rewrite Int64.add_zero_l. rewrite REGSAVEDSTK. *)
+(*   hexploit Mem.range_perm_free. *)
+(*   { eapply STKPERM. } intros [m2 FREE1]. *)
+(*   hexploit Mem.range_perm_free. *)
+(*   { instantiate (1:=0). *)
+(*     instantiate (1:=0). *)
+(*     instantiate (1:=initstk). *)
+(*     instantiate (1:=m2). *)
+(*     ii. omega. } intros [m4 FREE2]. *)
+(*   exists (nextinstr_nf rs0 # RBX <- (init_rs RBX)). eexists. eexists. *)
+(*   exists m2. exists m4. *)
+(*   replace ((nextinstr_nf rs0 # RBX <- (init_rs RBX) RSP)) with (rs0 RSP); cycle 1. *)
+(*   { unfold nextinstr_nf, nextinstr, undef_regs. *)
+(*     repeat (rewrite Pregmap.gso; clarify). } *)
+(*   rewrite RASAVED. rewrite RSPSAVED. rewrite RSPVAL. psimpl. zsimpl. *)
+(*   rewrite FREE1. rewrite FREE2. esplits; eauto. *)
+(*   replace (rs0 RAX) with *)
+(*       ((nextinstr *)
+(*           ((nextinstr_nf rs0 # RBX <- (init_rs RBX)) # RSP <- (init_rs RSP)) # RA <- *)
+(*           (init_rs RA)) # PC <- *)
+(*                         (nextinstr *)
+(*                            ((nextinstr_nf rs0 # RBX <- (init_rs RBX)) # RSP <- (init_rs RSP)) # RA <- *)
+(*                            (init_rs RA) RA) (to_preg Machregs.AX)); cycle 1. *)
+(*   { unfold nextinstr, Pregmap.set, to_mreg, to_preg, preg_of. des_ifs. } *)
+(*   econs; eauto. *)
+(*   - i. eapply Val.lessdef_same. destruct (Machregs.mreg_eq mr Machregs.BX). *)
+(*     + clarify. *)
+(*     + erewrite REGSAVED; eauto. *)
+(*       unfold nextinstr_nf, nextinstr, undef_regs, to_preg, preg_of, Pregmap.set. des_ifs. *)
+(*   - unfold nextinstr, Pregmap.set, to_mreg, to_preg, preg_of. des_ifs. *)
+(*     unfold external_state, Genv.find_funct, Genv.find_funct_ptr. des_ifs. *)
+(*     exfalso. eapply RANOTFPTR; eauto. eapply Genv.genv_defs_range in Heq2; eauto. *)
+(*   - unfold Genv.find_funct, Genv.find_funct_ptr. des_ifs. *)
+(*     exfalso. eapply RANOTFPTR; eauto. eapply Genv.genv_defs_range; eauto. *)
+(* Qed. *)
+
 
 Theorem sim_modsem
   :
     ModSemPair.sim msp
 .
 Proof.
-  admit "TODO".
+  econs; eauto.
+  { i. eapply SoundTop.sound_state_local_preservation. }
+  { i. eapply Preservation.local_preservation_noguarantee_weak; eauto. eapply SoundTop.sound_state_local_preservation. }
+  i. ss. esplits; eauto.
+
+  - i. des. inv SAFESRC. instantiate (1:=unit).
+    esplits; eauto.
+    + refl.
+    + econs; eauto.
+    + instantiate (1:= (Ord.lift_idx lt_wf 15%nat)).
+      inv INITTGT. inv TYP. ss.
+      assert (FD: fd = func_g).
+      { admit "genv". } clarify.
+
+      admit "see well_saved_initial".
+
+  - (* init progress *)
+    i.
+    des. inv SAFESRC.
+    inv SIMARGS; ss.
+
+    exploit asm_initial_frame_succeed; eauto.
+    + instantiate (1:=func_g). ss.
+      eapply inject_list_length in VALS. des. rewrite <- VALS.
+      rewrite VS. ss.
+    + ss.
+    + admit "genv".
 Qed.
 
 
